Update typing judgements and semantics

Typing.thy
@@ -1,166 +1,288 @@
 theory Typing
-  imports Syntax Defs Lemmas
+  imports Syntax Defs Lemmas "HOL-Eisbach.Eisbach" "HOL-Eisbach.Eisbach_Tools"
 begin
 
 no_notation Set.member  ("(_/ : _)" [51, 51] 50)
 
-inductive Ctx :: "\<Gamma> \<Rightarrow> bool" ("\<turnstile> _")
-  and Ty :: "\<Gamma> \<Rightarrow> \<tau> \<Rightarrow> \<kappa> \<Rightarrow> bool" ("_ \<turnstile>\<^sub>t\<^sub>y _ : _") where
+inductive Ax :: "\<Delta> \<Rightarrow> bool" ("\<turnstile> _")
+  and Ctx :: "\<Delta> \<Rightarrow> \<Gamma> \<Rightarrow> bool" ("_ \<turnstile> _")
+  and Ty :: "\<Gamma> \<Rightarrow> \<Delta> \<Rightarrow> \<tau> \<Rightarrow> \<kappa> \<Rightarrow> bool" ("_ , _ \<turnstile>\<^sub>t\<^sub>y _ : _") where
 
-  Ctx_Empty: "\<turnstile> []"
+  Ax_Empty: "\<turnstile> []"
 
-| Ctx_TyVar: "\<lbrakk> \<turnstile> \<Gamma> ; atom a \<sharp> \<Gamma> \<rbrakk> \<Longrightarrow> \<turnstile> BTyVar a k # \<Gamma>"
+| Ax_Data: "\<lbrakk> \<turnstile> \<Delta> ; atom T \<sharp> \<Delta> \<rbrakk> \<Longrightarrow> \<turnstile> AxData T \<kappa> # \<Delta>"
 
-| Ctx_Var: "\<lbrakk> \<Gamma> \<turnstile>\<^sub>t\<^sub>y \<tau> : \<star> ; atom x \<sharp> \<Gamma> \<rbrakk> \<Longrightarrow> \<turnstile> BVar x \<tau> # \<Gamma>"
+| Ax_Ctor: "\<lbrakk> [] , \<Delta> \<turnstile>\<^sub>t\<^sub>y \<tau> : \<star> ; atom D \<sharp> \<Delta> \<rbrakk> \<Longrightarrow> \<turnstile> AxCtor D \<tau> # \<Delta>"
 
 (* ------------------------------ *)
 
-| Ty_Var: "\<lbrakk> \<turnstile> \<Gamma> ; BTyVar a k \<in> \<Gamma> \<rbrakk> \<Longrightarrow> \<Gamma> \<turnstile>\<^sub>t\<^sub>y TyVar a : k"
+| Ctx_Empty: "\<turnstile> \<Delta> \<Longrightarrow> \<Delta> \<turnstile> []"
 
-| Ty_App: "\<lbrakk> \<Gamma> \<turnstile>\<^sub>t\<^sub>y \<tau>1 : KArrow \<kappa>1 \<kappa>2 ; \<Gamma> \<turnstile>\<^sub>t\<^sub>y \<tau>2 : \<kappa>1 \<rbrakk> \<Longrightarrow> \<Gamma> \<turnstile>\<^sub>t\<^sub>y TyConApp \<tau>1 \<tau>2 : \<kappa>2"
+| Ctx_TyVar: "\<lbrakk> \<Delta> \<turnstile> \<Gamma> ; atom a \<sharp> \<Gamma> \<rbrakk> \<Longrightarrow> \<Delta> \<turnstile> BTyVar a k # \<Gamma>"
 
-| Ty_Unit: "\<turnstile> \<Gamma> \<Longrightarrow> \<Gamma> \<turnstile>\<^sub>t\<^sub>y TyUnit : \<star>" (* to be replaced with ADTs *)
+| Ctx_Var: "\<lbrakk> \<Gamma> , \<Delta> \<turnstile>\<^sub>t\<^sub>y \<tau> : \<star> ; atom x \<sharp> \<Gamma> \<rbrakk> \<Longrightarrow> \<Delta> \<turnstile> BVar x \<tau> # \<Gamma>"
 
-| Ty_FunArrow: "\<lbrakk> \<Gamma> \<turnstile>\<^sub>t\<^sub>y \<tau>1 : \<star> ; \<Gamma> \<turnstile>\<^sub>t\<^sub>y \<tau>2 : \<star> \<rbrakk> \<Longrightarrow> \<Gamma> \<turnstile>\<^sub>t\<^sub>y (\<tau>1 \<rightarrow> \<tau>2) : \<star>" (* also to be a type constant *)
+(* ------------------------------ *)
 
-| Ty_Forall: "\<lbrakk> BTyVar a k # \<Gamma> \<turnstile>\<^sub>t\<^sub>y \<sigma> : \<star> \<rbrakk> \<Longrightarrow> \<Gamma> \<turnstile>\<^sub>t\<^sub>y (\<forall>a : k. \<sigma>) : \<star>"
+| Ty_Var: "\<lbrakk> \<Delta> \<turnstile> \<Gamma> ; BTyVar a k \<in> \<Gamma> \<rbrakk> \<Longrightarrow> \<Gamma> , \<Delta> \<turnstile>\<^sub>t\<^sub>y TyVar a : k"
 
-equivariance Ctx
+| Ty_App: "\<lbrakk> \<Gamma> , \<Delta> \<turnstile>\<^sub>t\<^sub>y \<tau>1 : \<kappa>1 \<rightarrow> \<kappa>2 ; \<Gamma> , \<Delta> \<turnstile>\<^sub>t\<^sub>y \<tau>2 : \<kappa>1 \<rbrakk> \<Longrightarrow> \<Gamma> , \<Delta> \<turnstile>\<^sub>t\<^sub>y TyApp \<tau>1 \<tau>2 : \<kappa>2"
 
-inductive Tm :: "\<Gamma> \<Rightarrow> term \<Rightarrow> \<tau> \<Rightarrow> bool" ("_ \<turnstile> _ : _" 50) where
-  Tm_Var: "\<lbrakk> \<turnstile> \<Gamma> ; BVar x \<tau> \<in> \<Gamma> \<rbrakk> \<Longrightarrow> \<Gamma> \<turnstile> (Var x) : \<tau>"
+| Ty_Data: "\<lbrakk> \<Delta> \<turnstile> \<Gamma> ; AxData T k \<in> set \<Delta> \<rbrakk> \<Longrightarrow> \<Gamma> , \<Delta> \<turnstile>\<^sub>t\<^sub>y TyData T TNil : k"
 
-| Tm_Abs: "BVar x \<tau>1 # \<Gamma> \<turnstile> e : \<tau>2 \<Longrightarrow> \<Gamma> \<turnstile> (\<lambda> x : \<tau>1 . e) : (\<tau>1 \<rightarrow> \<tau>2)"
+| Ty_DataApp: "\<Gamma> , \<Delta> \<turnstile>\<^sub>t\<^sub>y TyApp (TyData T tys) \<tau>2 : k \<Longrightarrow> \<Gamma> , \<Delta> \<turnstile>\<^sub>t\<^sub>y TyData T (TCons \<tau>2 tys) : k"
 
-| Tm_App: "\<lbrakk> \<Gamma> \<turnstile> e1 : (\<tau>1 \<rightarrow> \<tau>2) ; \<Gamma> \<turnstile> e2 : \<tau>1 \<rbrakk> \<Longrightarrow> \<Gamma> \<turnstile> App e1 e2 : \<tau>2"
+| Ty_Arrow: "\<Delta> \<turnstile> \<Gamma> \<Longrightarrow> \<Gamma> , \<Delta> \<turnstile>\<^sub>t\<^sub>y TyArrow : \<star> \<rightarrow> \<star> \<rightarrow> \<star>"
 
-| Tm_TAbs: "BTyVar a k # \<Gamma> \<turnstile> e : \<sigma> \<Longrightarrow> \<Gamma> \<turnstile> (\<Lambda> a : k . e) : (\<forall> a : k . \<sigma>)"
+| Ty_Forall: "\<lbrakk> BTyVar a k # \<Gamma> , \<Delta> \<turnstile>\<^sub>t\<^sub>y \<sigma> : \<star> \<rbrakk> \<Longrightarrow> \<Gamma> , \<Delta> \<turnstile>\<^sub>t\<^sub>y (\<forall>a : k. \<sigma>) : \<star>"
 
-| Tm_TApp: "\<lbrakk> \<Gamma> \<turnstile> e : \<forall> a:k. \<sigma> ; \<Gamma> \<turnstile>\<^sub>t\<^sub>y \<tau> : k \<rbrakk> \<Longrightarrow> \<Gamma> \<turnstile> TyApp e \<tau> : \<sigma>[\<tau>/a]"
+method solve_Ax_Ctx_Ty = (
+  rule Ty_Arrow, print_fact Ty_Arrow
+  | match conclusion in
+    "\<turnstile> []" \<Rightarrow> \<open>print_fact Ax_Empty, rule Ax_Empty\<close>
+    \<bar> "\<turnstile> AxData _ _ # _" \<Rightarrow> \<open>print_fact Ax_Data, rule Ax_Data\<close>
+    \<bar> "\<turnstile> AxCtor _ _ # _" \<Rightarrow> \<open>print_fact Ax_Ctor, rule Ax_Ctor\<close>
+    \<bar> "_ \<turnstile> BTyVar _ _ # _" \<Rightarrow> \<open>print_fact Ctx_TyVar, rule Ctx_TyVar\<close>
+    \<bar> "(_::\<Delta>) \<turnstile> []" \<Rightarrow> \<open>print_fact Ctx_Empty, rule Ctx_Empty\<close>
+    \<bar> "_ , _ \<turnstile>\<^sub>t\<^sub>y TyForall _ _ _ : _" \<Rightarrow> \<open>print_fact Ty_Forall, rule Ty_Forall\<close>
+    \<bar> "_ , _ \<turnstile>\<^sub>t\<^sub>y TyData _ (TCons _ _) : _" \<Rightarrow> \<open>print_fact Ty_DataApp, rule Ty_DataApp\<close>
+    \<bar> "_ , _ \<turnstile>\<^sub>t\<^sub>y TyData _ TNil : _" \<Rightarrow> \<open>print_fact Ty_Data, rule Ty_Data\<close>
+    \<bar> "_ , _ \<turnstile>\<^sub>t\<^sub>y TyApp _ _ : _" \<Rightarrow> \<open>print_fact Ty_App, rule Ty_App\<close>
+    \<bar> "_ , _ \<turnstile>\<^sub>t\<^sub>y TyVar _ : _" \<Rightarrow> \<open>print_fact Ty_Var, rule Ty_Var\<close>
+    \<bar> "_ \<sharp> []" \<Rightarrow> \<open>print_fact fresh_Nil, rule fresh_Nil\<close>
+  | (simp add: fresh_Nil fresh_Cons)
+  | (simp add: fresh_at_base Abs_ctor_name_inject Abs_data_name_inject)
+)+
 
-| Tm_Unit: "\<turnstile> \<Gamma> \<Longrightarrow> \<Gamma> \<turnstile> Unit : TyUnit" (* to be replaced with ADTs *)
+abbreviation mkCtor :: "nat \<Rightarrow> ctor_name" where
+  "mkCtor n \<equiv> Abs_ctor_name (Atom (Sort ''Syntax.ctor_name'' []) n)"
 
-| Tm_Let: "\<lbrakk> \<Gamma> \<turnstile> e1 : \<tau>1 ; BVar x \<tau>1 # \<Gamma> \<turnstile> e2 : \<tau>2 \<rbrakk> \<Longrightarrow> \<Gamma> \<turnstile> Let x \<tau>1 e1 e2 : \<tau>2"
+abbreviation mkData :: "nat \<Rightarrow> data_name" where
+  "mkData n \<equiv> Abs_data_name (Atom (Sort ''Syntax.data_name'' []) n)"
+
+(* data Maybe a = Nothing | Just a *)
+lemma "\<turnstile> [
+  AxCtor (mkCtor 2) (\<forall> a:\<star> . TyVar a \<rightarrow> TyData (mkData 0) (TCons (TyVar a) TNil)),
+  AxCtor (mkCtor 1) (\<forall> a:\<star> . TyData (mkData 0) (TCons (TyVar a) TNil) ),
+  AxData (mkData 0) (\<star> \<rightarrow> \<star>)
+]" (* 0: Maybe, 1: Nothing, 2: Just *)
+  by solve_Ax_Ctx_Ty
+
+equivariance Ax
+
+inductive Tm :: "\<Gamma> \<Rightarrow> \<Delta> \<Rightarrow> term \<Rightarrow> \<tau> \<Rightarrow> bool" ("_ , _ \<turnstile> _ : _" 50) where
+  Tm_Var: "\<lbrakk> \<Delta> \<turnstile> \<Gamma> ; BVar x \<tau> \<in> \<Gamma> \<rbrakk> \<Longrightarrow> \<Gamma> , \<Delta> \<turnstile> (Var x) : \<tau>"
+
+| Tm_Abs: "BVar x \<tau>1 # \<Gamma> , \<Delta> \<turnstile> e : \<tau>2 \<Longrightarrow> \<Gamma> , \<Delta> \<turnstile> (\<lambda> x : \<tau>1 . e) : (\<tau>1 \<rightarrow> \<tau>2)"
+
+| Tm_App: "\<lbrakk> \<Gamma> , \<Delta> \<turnstile> e1 : (\<tau>1 \<rightarrow> \<tau>2) ; \<Gamma> , \<Delta> \<turnstile> e2 : \<tau>1 \<rbrakk> \<Longrightarrow> \<Gamma> , \<Delta> \<turnstile> App e1 e2 : \<tau>2"
+
+| Tm_TAbs: "BTyVar a k # \<Gamma> , \<Delta> \<turnstile> e : \<sigma> \<Longrightarrow> \<Gamma> , \<Delta> \<turnstile> (\<Lambda> a : k . e) : (\<forall> a : k . \<sigma>)"
+
+| Tm_TApp: "\<lbrakk> \<Gamma> , \<Delta> \<turnstile> e : \<forall> a:k. \<sigma> ; \<Gamma> , \<Delta> \<turnstile>\<^sub>t\<^sub>y \<tau> : k \<rbrakk> \<Longrightarrow> \<Gamma> , \<Delta> \<turnstile> TApp e \<tau> : \<sigma>[\<tau>/a]"
+
+| Tm_DataCon: "\<lbrakk> \<Delta> \<turnstile> \<Gamma> ; AxCtor D \<tau> \<in> set \<Delta> \<rbrakk> \<Longrightarrow> \<Gamma> , \<Delta> \<turnstile> Ctor D TNil ENil : \<tau>"
+
+| Tm_DataConApp: "\<Gamma> , \<Delta> \<turnstile> App (Ctor D tys vals) e : \<tau> \<Longrightarrow> \<Gamma> , \<Delta> \<turnstile> Ctor D tys (ECons e vals) : \<tau>"
+
+| Tm_DataConTApp: "\<Gamma> , \<Delta> \<turnstile> TApp (Ctor D tys vals) \<sigma> : \<tau> \<Longrightarrow> \<Gamma> , \<Delta> \<turnstile> Ctor D (TCons \<sigma> tys) vals : \<tau>"
+
+| Tm_Let: "\<lbrakk> \<Gamma> , \<Delta> \<turnstile> e1 : \<tau>1 ; BVar x \<tau>1 # \<Gamma> , \<Delta> \<turnstile> e2 : \<tau>2 \<rbrakk> \<Longrightarrow> \<Gamma> , \<Delta> \<turnstile> Let x \<tau>1 e1 e2 : \<tau>2"
 
 equivariance Tm
 
-lemmas Ctx_intros = Ctx_Ty.intros(1-3)
-lemmas Ty_intros = Ctx_Ty.intros(4-8)
+lemmas Ax_intros = Ax_Ctx_Ty.intros(1-3)
+lemmas Ctx_intros = Ax_Ctx_Ty.intros(4-6)
+lemmas Ty_intros = Ax_Ctx_Ty.intros(7-11)
+
+inductive_cases AxE[elim]:
+  "\<turnstile> AxData T k # \<Delta>"
+  "\<turnstile> AxCtor D \<tau> # \<Delta>"
 
 inductive_cases CtxE[elim]:
-  "\<turnstile> BTyVar a k # \<Gamma>"
-  "\<turnstile> BVar x \<tau> # \<Gamma>"
+  "\<Delta> \<turnstile> BTyVar a k # \<Gamma>"
+  "\<Delta> \<turnstile> BVar x \<tau> # \<Gamma>"
 
 inductive_cases TyE[elim!]:
-  "\<Gamma> \<turnstile>\<^sub>t\<^sub>y TyVar a : k"
-  "\<Gamma> \<turnstile>\<^sub>t\<^sub>y TyConApp \<tau>1 \<tau>2 : \<kappa>2"
-  "\<Gamma> \<turnstile>\<^sub>t\<^sub>y TyUnit : k"
-  "\<Gamma> \<turnstile>\<^sub>t\<^sub>y (\<tau>1 \<rightarrow> \<tau>2) : k"
+  "\<Gamma> , \<Delta> \<turnstile>\<^sub>t\<^sub>y TyVar a : k"
+  "\<Gamma> , \<Delta> \<turnstile>\<^sub>t\<^sub>y TyApp \<tau>1 \<tau>2 : \<kappa>2"
+  "\<Gamma> , \<Delta> \<turnstile>\<^sub>t\<^sub>y TyData D tys : k"
+  "\<Gamma> , \<Delta> \<turnstile>\<^sub>t\<^sub>y TyArrow : k"
 
 inductive_cases TmE[elim!]:
-  "\<Gamma> \<turnstile> (Var x) : \<tau>"
-  "\<Gamma> \<turnstile> App e1 e2 : \<tau>2"
-  "\<Gamma> \<turnstile> TyApp e \<tau> : \<sigma>[\<tau>/a]"
-  "\<Gamma> \<turnstile> Unit : \<tau>"
+  "\<Gamma> , \<Delta> \<turnstile> (Var x) : \<tau>"
+  "\<Gamma> , \<Delta> \<turnstile> App e1 e2 : \<tau>2"
+  "\<Gamma> , \<Delta> \<turnstile> TApp e \<tau> : \<tau>2"
+  "\<Gamma> , \<Delta> \<turnstile> Ctor D tys vals : \<tau>"
 
 (* Split induction principles *)
+lemma Ax_induct[consumes 1, case_names Empty Data Ctor]:
+  assumes "\<turnstile> \<Delta>"
+  and "P []"
+  and "\<And>T \<Delta> \<kappa>. \<lbrakk> \<turnstile> \<Delta> ; P \<Delta> ; atom T \<sharp> \<Delta> \<rbrakk> \<Longrightarrow> P (AxData T \<kappa> # \<Delta>)"
+  and "\<And>\<Delta> \<tau> D. \<lbrakk> [] , \<Delta> \<turnstile>\<^sub>t\<^sub>y \<tau> : \<star> ; atom D \<sharp> \<Delta> \<rbrakk> \<Longrightarrow> P (AxCtor D \<tau> # \<Delta>)"
+shows "P \<Delta>"
+  using Ax_Ctx_Ty.inducts(1)[OF assms(1), of P "\<lambda>a b c d. True" "\<lambda>a b. True"] assms(2-4) by simp
+
 lemma Ctx_induct[consumes 1, case_names Empty TyVar Var]:
-  assumes "\<turnstile> \<Gamma>"
-  and Empty: "P []"
-  and TyVar: "\<And>\<Gamma> a k. \<lbrakk> \<turnstile> \<Gamma> ; P \<Gamma> ; atom a \<sharp> \<Gamma> \<rbrakk> \<Longrightarrow> P (BTyVar a k # \<Gamma>)"
-  and Var: "\<And>\<Gamma> x \<tau>. \<lbrakk> \<Gamma> \<turnstile>\<^sub>t\<^sub>y \<tau> : \<star> ; atom x \<sharp> \<Gamma> \<rbrakk> \<Longrightarrow> P (BVar x \<tau> # \<Gamma>)"
-shows "P \<Gamma>"
-  using assms(1) by (induction \<Gamma> rule: Ctx_Ty.inducts(1)) (auto simp: assms)
+  fixes \<Delta>::"\<Delta>"
+  assumes "\<Delta> \<turnstile> \<Gamma>"
+  and Empty: "\<And>\<Delta>. P \<Delta> []"
+  and TyVar: "\<And>\<Delta> \<Gamma> a k. \<lbrakk> \<Delta> \<turnstile> \<Gamma> ; P \<Delta> \<Gamma> ; atom a \<sharp> \<Gamma> \<rbrakk> \<Longrightarrow> P \<Delta> (BTyVar a k # \<Gamma>)"
+  and Var: "\<And>\<Gamma> \<Delta> x \<tau>. \<lbrakk> \<Gamma> , \<Delta> \<turnstile>\<^sub>t\<^sub>y \<tau> : \<star> ; atom x \<sharp> \<Gamma> \<rbrakk> \<Longrightarrow> P \<Delta> (BVar x \<tau> # \<Gamma>)"
+shows "P \<Delta> \<Gamma>"
+  using Ax_Ctx_Ty.inducts(2)[OF assms(1), of "\<lambda>x. True" "\<lambda>a b c d. True" P] assms(2-4) by simp
 
-lemma Ty_induct[consumes 1, case_names Var App Unit FunArrow Forall]:
-  assumes "\<Gamma> \<turnstile>\<^sub>t\<^sub>y \<tau> : \<kappa>"
-  and Var: "\<And>\<Gamma> a k. \<lbrakk> \<turnstile> \<Gamma> ; BTyVar a k \<in> \<Gamma> \<rbrakk> \<Longrightarrow> P \<Gamma> (TyVar a) k"
-  and App: "\<And>\<Gamma> \<tau>1 \<tau>2 \<kappa>1 \<kappa>2. \<lbrakk> \<Gamma> \<turnstile>\<^sub>t\<^sub>y \<tau>1 : KArrow \<kappa>1 \<kappa>2 ; P \<Gamma> \<tau>1 (KArrow \<kappa>1 \<kappa>2) ; \<Gamma> \<turnstile>\<^sub>t\<^sub>y \<tau>2 : \<kappa>1 ; P \<Gamma> \<tau>2 \<kappa>1 \<rbrakk> \<Longrightarrow> P \<Gamma> (TyConApp \<tau>1 \<tau>2) \<kappa>2"
-  and Unit: "\<And>\<Gamma>. \<turnstile> \<Gamma> \<Longrightarrow> P \<Gamma> TyUnit \<star>"
-  and FunArrow: "\<And>\<Gamma> \<tau>1 \<tau>2. \<lbrakk> \<Gamma> \<turnstile>\<^sub>t\<^sub>y \<tau>1 : \<star> ; P \<Gamma> \<tau>1 \<star> ; \<Gamma> \<turnstile>\<^sub>t\<^sub>y \<tau>2 : \<star> ; P \<Gamma> \<tau>2 \<star> \<rbrakk> \<Longrightarrow> P \<Gamma> (\<tau>1 \<rightarrow> \<tau>2) \<star>"
-  and Forall: "\<And>\<Gamma> a k \<sigma>. \<lbrakk> BTyVar a k # \<Gamma> \<turnstile>\<^sub>t\<^sub>y \<sigma> : \<star> ; P (BTyVar a k # \<Gamma>) \<sigma> \<star> \<rbrakk> \<Longrightarrow> P \<Gamma> (\<forall> a:k. \<sigma>) \<star>"
-shows "P \<Gamma> \<tau> \<kappa>"
-  using assms(1) by (induction \<Gamma> \<tau> \<kappa> rule: Ctx_Ty.inducts(2)) (auto simp: assms)
+thm Ax_Ctx_Ty.inducts(3)
 
-lemma Ctx_Ty_induct_split[case_names Ctx_Empty Ctx_TyVar Ctx_Var Ty_Var Ty_App Ty_Unit Ty_FunArrow Ty_Forall]:
-  assumes "P []"
-  and "\<And>\<Gamma>' b k2. \<lbrakk> \<turnstile> \<Gamma>' @ \<Gamma> ; P \<Gamma>' ; atom b \<sharp> \<Gamma>' @  \<Gamma> \<rbrakk> \<Longrightarrow> P (BTyVar b k2 # \<Gamma>')"
-  and "\<And>\<Gamma>' \<tau> x. \<lbrakk> \<Gamma>' @ \<Gamma> \<turnstile>\<^sub>t\<^sub>y \<tau> : \<star> ; Q \<Gamma>' \<tau> \<star> ; atom x \<sharp> \<Gamma>' @  \<Gamma> \<rbrakk> \<Longrightarrow> P (BVar x \<tau> # \<Gamma>')"
-  and "\<And>\<Gamma>' b k2. \<lbrakk> \<turnstile> \<Gamma>' @ \<Gamma> ; P \<Gamma>' ; BTyVar b k2 \<in> (\<Gamma>' @  \<Gamma>) \<rbrakk> \<Longrightarrow> Q \<Gamma>' (TyVar b) k2"
-  and "\<And>\<Gamma>' \<tau>1 \<kappa>1 \<kappa>2 \<tau>2. \<lbrakk> \<Gamma>' @ \<Gamma> \<turnstile>\<^sub>t\<^sub>y \<tau>1 : KArrow \<kappa>1 \<kappa>2 ; Q \<Gamma>' \<tau>1 (KArrow \<kappa>1 \<kappa>2) ; \<Gamma>' @ \<Gamma> \<turnstile>\<^sub>t\<^sub>y \<tau>2 : \<kappa>1 ; Q \<Gamma>' \<tau>2 \<kappa>1 \<rbrakk> \<Longrightarrow> Q \<Gamma>' (TyConApp \<tau>1 \<tau>2) \<kappa>2"
-  and "\<And>\<Gamma>'. \<lbrakk> \<turnstile> \<Gamma>' @ \<Gamma> ; P \<Gamma>' \<rbrakk> \<Longrightarrow> Q \<Gamma>' TyUnit \<star>"
-  and "\<And>\<Gamma>' \<tau>1 \<tau>2. \<lbrakk> \<Gamma>' @ \<Gamma> \<turnstile>\<^sub>t\<^sub>y \<tau>1 : \<star> ; Q \<Gamma>' \<tau>1 \<star> ; \<Gamma>' @  \<Gamma> \<turnstile>\<^sub>t\<^sub>y \<tau>2 : \<star> ; Q \<Gamma>' \<tau>2 \<star> \<rbrakk> \<Longrightarrow> Q \<Gamma>' (\<tau>1 \<rightarrow> \<tau>2) \<star>"
-  and "\<And>b k2 \<Gamma>' \<sigma>. \<lbrakk> BTyVar b k2 # \<Gamma>' @ \<Gamma> \<turnstile>\<^sub>t\<^sub>y \<sigma> : \<star> ; Q (BTyVar b k2 # \<Gamma>') \<sigma> \<star> \<rbrakk> \<Longrightarrow> Q \<Gamma>' (\<forall> b : k2 . \<sigma>) \<star>"
-shows "\<turnstile> \<Gamma>' @ \<Gamma> \<longrightarrow> P \<Gamma>'"
-  and "\<Gamma>' @ \<Gamma> \<turnstile>\<^sub>t\<^sub>y \<tau> : k2 \<longrightarrow> Q \<Gamma>' \<tau> k2"
+lemma Ty_induct[consumes 1, case_names Var App Data DataApp Arrow Forall]:
+  fixes P::"\<Gamma> \<Rightarrow> \<Delta> \<Rightarrow> \<tau> \<Rightarrow> \<kappa> \<Rightarrow> bool"
+  assumes "\<Gamma> , \<Delta> \<turnstile>\<^sub>t\<^sub>y \<tau> : \<kappa>"
+  and Var: "\<And>\<Gamma> \<Delta> a k. \<lbrakk> \<Delta> \<turnstile> \<Gamma> ; BTyVar a k \<in> \<Gamma> \<rbrakk> \<Longrightarrow> P \<Gamma> \<Delta> (TyVar a) k"
+  and App: "\<And>\<Gamma> \<Delta> \<tau>1 \<tau>2 \<kappa>1 \<kappa>2. \<lbrakk> \<Gamma> , \<Delta> \<turnstile>\<^sub>t\<^sub>y \<tau>1 : \<kappa>1 \<rightarrow> \<kappa>2 ; P \<Gamma> \<Delta> \<tau>1 (KArrow \<kappa>1 \<kappa>2) ; \<Gamma> , \<Delta> \<turnstile>\<^sub>t\<^sub>y \<tau>2 : \<kappa>1 ; P \<Gamma> \<Delta> \<tau>2 \<kappa>1 \<rbrakk> \<Longrightarrow> P \<Gamma> \<Delta> (TyApp \<tau>1 \<tau>2) \<kappa>2"
+  and Data: "\<And>\<Delta> \<Gamma> T k. \<lbrakk> \<Delta> \<turnstile> \<Gamma> ; AxData T k \<in> set \<Delta> \<rbrakk> \<Longrightarrow> P \<Gamma> \<Delta> (TyData T TNil) k"
+  and DataApp: "\<And>\<Gamma> \<Delta> T tys \<tau>2 k. \<lbrakk> \<Gamma> , \<Delta> \<turnstile>\<^sub>t\<^sub>y TyApp (TyData T tys) \<tau>2 : k ; P \<Gamma> \<Delta> (TyApp (TyData T tys) \<tau>2) k \<rbrakk> \<Longrightarrow> P \<Gamma> \<Delta> (TyData T (TCons \<tau>2 tys)) k"
+  and Arrow: "\<And>\<Gamma> \<Delta>. \<Delta> \<turnstile> \<Gamma> \<Longrightarrow> P \<Gamma> \<Delta> TyArrow (\<star> \<rightarrow> \<star> \<rightarrow> \<star>)"
+  and Forall: "\<And>\<Gamma> \<Delta> a k \<sigma>. \<lbrakk> BTyVar a k # \<Gamma> , \<Delta> \<turnstile>\<^sub>t\<^sub>y \<sigma> : \<star> ; P (BTyVar a k # \<Gamma>) \<Delta> \<sigma> \<star> \<rbrakk> \<Longrightarrow> P \<Gamma> \<Delta> (\<forall> a:k. \<sigma>) \<star>"
+shows "P \<Gamma> \<Delta> \<tau> \<kappa>"
+  using Ax_Ctx_Ty.inducts(3)[OF assms(1), of "\<lambda>a. True" P "\<lambda>a b. True"] assms(2-7) by simp
+
+lemma Ctx_Ty_induct_split[case_names Ctx_Empty Ctx_TyVar Ctx_Var Ty_Var Ty_App Ty_Data Ty_DataApp Ty_Arrow Ty_Forall]:
+  fixes P::"\<Delta> \<Rightarrow> \<Gamma> \<Rightarrow> bool" and Q::"\<Gamma> \<Rightarrow> \<Delta> \<Rightarrow> \<tau> \<Rightarrow> \<kappa> \<Rightarrow> bool"
+  assumes "\<And>\<Delta>. P \<Delta> []"
+  and "\<And>\<Gamma>' \<Delta> b k2. \<lbrakk> \<Delta> \<turnstile> \<Gamma>' @ \<Gamma> ; P \<Delta> \<Gamma>' ; atom b \<sharp> (\<Gamma>' @  \<Gamma>) \<rbrakk> \<Longrightarrow> P \<Delta> (BTyVar b k2 # \<Gamma>')"
+  and "\<And>\<Gamma>' \<Delta> \<tau> x. \<lbrakk> \<Gamma>' @ \<Gamma> , \<Delta> \<turnstile>\<^sub>t\<^sub>y \<tau> : \<star> ; Q \<Gamma>' \<Delta> \<tau> \<star> ; atom x \<sharp> (\<Gamma>' @  \<Gamma>) \<rbrakk> \<Longrightarrow> P \<Delta> (BVar x \<tau> # \<Gamma>')"
+  and "\<And>\<Gamma>' \<Delta> b k2. \<lbrakk> \<Delta> \<turnstile> \<Gamma>' @ \<Gamma> ; P \<Delta> \<Gamma>' ; BTyVar b k2 \<in> (\<Gamma>' @  \<Gamma>) \<rbrakk> \<Longrightarrow> Q \<Gamma>' \<Delta> (TyVar b) k2"
+  and "\<And>\<Gamma>' \<Delta> \<tau>1 \<kappa>1 \<kappa>2 \<tau>2. \<lbrakk> \<Gamma>' @ \<Gamma> , \<Delta> \<turnstile>\<^sub>t\<^sub>y \<tau>1 : \<kappa>1 \<rightarrow> \<kappa>2 ; Q \<Gamma>' \<Delta> \<tau>1 (\<kappa>1 \<rightarrow> \<kappa>2) ; \<Gamma>' @ \<Gamma> , \<Delta> \<turnstile>\<^sub>t\<^sub>y \<tau>2 : \<kappa>1 ; Q \<Gamma>' \<Delta> \<tau>2 \<kappa>1 \<rbrakk> \<Longrightarrow> Q \<Gamma>' \<Delta> (TyApp \<tau>1 \<tau>2) \<kappa>2"
+  and "\<And>\<Gamma>' \<Delta> T k. \<lbrakk> \<Delta> \<turnstile> \<Gamma>' @ \<Gamma> ; AxData T k \<in> set \<Delta> \<rbrakk> \<Longrightarrow> Q \<Gamma>' \<Delta> (TyData T TNil) k"
+  and "\<And>\<Gamma>' \<Delta> T tys \<tau>2 k. \<lbrakk> \<Gamma>' @ \<Gamma> , \<Delta> \<turnstile>\<^sub>t\<^sub>y TyApp (TyData T tys) \<tau>2 : k ; Q \<Gamma>' \<Delta> (TyApp (TyData T tys) \<tau>2) k \<rbrakk> \<Longrightarrow> Q \<Gamma>' \<Delta> (TyData T (TCons \<tau>2 tys)) k"
+  and "\<And>\<Gamma>' \<Delta>. \<lbrakk> \<Delta> \<turnstile> (\<Gamma>' @ \<Gamma>) ; P \<Delta> \<Gamma>' \<rbrakk> \<Longrightarrow> Q \<Gamma>' \<Delta> TyArrow (\<star> \<rightarrow> \<star> \<rightarrow> \<star>)"
+  and "\<And>\<Gamma>' \<Delta> b k2 \<sigma>. \<lbrakk> BTyVar b k2 # \<Gamma>' @ \<Gamma> , \<Delta> \<turnstile>\<^sub>t\<^sub>y \<sigma> : \<star> ; Q (BTyVar b k2 # \<Gamma>') \<Delta> \<sigma> \<star> \<rbrakk> \<Longrightarrow> Q \<Gamma>' \<Delta> (\<forall> b : k2 . \<sigma>) \<star>"
+shows "\<Delta> \<turnstile> \<Gamma>' @ \<Gamma> \<longrightarrow> P \<Delta> \<Gamma>'"
+  and "\<Gamma>' @ \<Gamma> , \<Delta> \<turnstile>\<^sub>t\<^sub>y \<tau> : k2 \<longrightarrow> Q \<Gamma>' \<Delta> \<tau> k2"
 proof -
   let ?\<Gamma> = "\<Gamma>' @ \<Gamma>"
-  let ?P = "\<lambda>x. \<forall>\<Gamma>2. (x = \<Gamma>2 @ \<Gamma>) \<longrightarrow> (P \<Gamma>2)"
-  let ?Q = "\<lambda>x y z. \<forall>\<Gamma>2. (x = \<Gamma>2 @ \<Gamma>) \<longrightarrow> (Q \<Gamma>2 y z)"
+  let ?P = "\<lambda>\<Delta> x. \<forall>\<Gamma>2. (x = \<Gamma>2 @ \<Gamma>) \<longrightarrow> (P \<Delta> \<Gamma>2)"
+  let ?Q = "\<lambda>x \<Delta> y z. \<forall>\<Gamma>2. (x = \<Gamma>2 @ \<Gamma>) \<longrightarrow> (Q \<Gamma>2 \<Delta> y z)"
 
-  have "(\<turnstile> ?\<Gamma> \<longrightarrow> ?P ?\<Gamma>) \<and> (?\<Gamma> \<turnstile>\<^sub>t\<^sub>y \<tau> : k2 \<longrightarrow> ?Q ?\<Gamma> \<tau> k2)"
-    apply (cases rule: Ctx_Ty.induct[of "?P" "?Q"]) apply auto
-  proof (cases)
-    fix \<Gamma>2' b \<kappa> \<Gamma>2
-    assume a: "\<turnstile> \<Gamma>2'" "\<forall>\<Gamma>2. \<Gamma>2' = \<Gamma>2 @ \<Gamma> \<longrightarrow> P \<Gamma>2" "atom b \<sharp> \<Gamma>2'" "BTyVar b \<kappa> # \<Gamma>2' = \<Gamma>2 @ \<Gamma>"
-    show "P \<Gamma>2"
-    proof (cases "\<Gamma>2 = []")
-      case False
-      then obtain G where "\<Gamma>2' = G @ \<Gamma>" by (meson Cons_eq_append_conv a(4))
-      then show ?thesis using assms(2) a by auto
-    qed (simp add: assms(1))
+  have "(\<turnstile> \<Delta> \<longrightarrow> True) \<and> (\<Delta> \<turnstile> ?\<Gamma> \<longrightarrow> ?P \<Delta> ?\<Gamma>) \<and> (?\<Gamma> , \<Delta> \<turnstile>\<^sub>t\<^sub>y \<tau> : k2 \<longrightarrow> ?Q ?\<Gamma> \<Delta> \<tau> k2)"
+  proof (cases rule: Ax_Ctx_Ty.induct[of "\<lambda>x. True" "?Q" "?P"])
+    case (Ctx_TyVar \<Delta> \<Gamma>' a k)
+    then show ?case
+    proof auto
+      fix \<Gamma>2
+      assume a: "BTyVar a k # \<Gamma>' = \<Gamma>2 @ \<Gamma>"
+      then show "P \<Delta> \<Gamma>2"
+      proof (cases "\<Gamma>2 = []")
+        case False
+        then obtain G where "\<Gamma>' = G @ \<Gamma>" by (meson Cons_eq_append_conv a)
+        then show ?thesis using assms(2) Ctx_TyVar a by auto
+      qed (simp add: assms(1))
+    qed
   next
-    fix \<Gamma>2' \<tau>2 x \<Gamma>2
-    assume a: "\<Gamma>2' \<turnstile>\<^sub>t\<^sub>y \<tau>2 : \<star>" "\<forall>\<Gamma>2. \<Gamma>2' = \<Gamma>2 @ \<Gamma> \<longrightarrow> Q \<Gamma>2 \<tau>2 \<star>" "atom x \<sharp> \<Gamma>2'" "BVar x \<tau>2 # \<Gamma>2' = \<Gamma>2 @ \<Gamma>"
-    show "P \<Gamma>2"
-    proof (cases "\<Gamma>2 = []")
-      case False
-      then obtain G where "\<Gamma>2' = G @ \<Gamma>" by (meson Cons_eq_append_conv a(4))
-      then show ?thesis using assms(3) a by auto
-    qed (simp add: assms(1))
-  qed (auto simp: assms(1,4-8))
-  then show "\<turnstile> \<Gamma>' @ \<Gamma> \<longrightarrow> P \<Gamma>'" and "\<Gamma>' @ \<Gamma> \<turnstile>\<^sub>t\<^sub>y \<tau> : k2 \<longrightarrow> Q \<Gamma>' \<tau> k2" by simp_all
+    case (Ctx_Var \<Gamma>' \<Delta> \<tau> x)
+    then show ?case
+    proof auto
+      fix \<Gamma>2
+      assume a: "BVar x \<tau> # \<Gamma>' = \<Gamma>2 @ \<Gamma>"
+      then show "P \<Delta> \<Gamma>2"
+      proof (cases "\<Gamma>2 = []")
+        case False
+        then obtain G where "\<Gamma>' = G @ \<Gamma>" by (meson Cons_eq_append_conv a)
+        then show ?thesis using assms(3) Ctx_Var a by auto
+      qed (simp add: assms(1))
+    qed
+  next
+    case (Ty_DataApp \<Gamma>' \<Delta> T tys \<tau>2 k)
+    show ?case
+    proof auto
+      fix \<Gamma>2
+      assume a: "\<Gamma>' = \<Gamma>2 @ \<Gamma>"
+      then have 1: "\<Gamma>2 @ \<Gamma> , \<Delta> \<turnstile>\<^sub>t\<^sub>y TyApp (TyData T tys) \<tau>2 : k" using Ty_DataApp(1) by simp
+      show "Q \<Gamma>2 \<Delta> (TyData T (TCons \<tau>2 tys)) k" using assms(7)[OF 1] a Ty_DataApp(2) by blast
+    qed
+  qed (auto simp: assms(1,4-9))
+
+  then show "\<Delta> \<turnstile> \<Gamma>' @ \<Gamma> \<longrightarrow> P \<Delta> \<Gamma>'" and "\<Gamma>' @ \<Gamma> , \<Delta> \<turnstile>\<^sub>t\<^sub>y \<tau> : k2 \<longrightarrow> Q \<Gamma>' \<Delta> \<tau> k2" by simp_all
 qed
 
+(* axiom validity *)
+lemma axioms_valid_aux:
+  shows "\<Delta> \<turnstile> \<Gamma> \<longrightarrow> \<turnstile> \<Delta>"
+  and "\<Gamma> , \<Delta> \<turnstile>\<^sub>t\<^sub>y \<tau> : k \<longrightarrow> \<turnstile> \<Delta>"
+proof -
+  have "(\<turnstile> \<Delta> \<longrightarrow> \<turnstile> \<Delta>) \<and> (\<Delta> \<turnstile> \<Gamma> \<longrightarrow> \<turnstile> \<Delta>) \<and> (\<Gamma> , \<Delta> \<turnstile>\<^sub>t\<^sub>y \<tau> : k \<longrightarrow> \<turnstile> \<Delta>)"
+    by (induction rule: Ax_Ctx_Ty.induct) (auto intro: Ax_intros)
+  then show "\<Delta> \<turnstile> \<Gamma> \<longrightarrow> \<turnstile> \<Delta>" and "\<Gamma> , \<Delta> \<turnstile>\<^sub>t\<^sub>y \<tau> : k \<longrightarrow> \<turnstile> \<Delta>" by simp_all
+qed
+lemma axioms_valid_context: "\<Delta> \<turnstile> \<Gamma> \<Longrightarrow> \<turnstile> \<Delta>"
+  using axioms_valid_aux by simp
+lemma axioms_valid_ty: "\<Gamma> , \<Delta> \<turnstile>\<^sub>t\<^sub>y \<tau> : k \<Longrightarrow> \<turnstile> \<Delta>"
+  using axioms_valid_aux by simp
+lemma axioms_valid_tm: "\<Gamma> , \<Delta> \<turnstile> e : \<tau> \<Longrightarrow> \<turnstile> \<Delta>"
+  by (induction \<Gamma> \<Delta> e \<tau> rule: Tm.induct) (auto simp: axioms_valid_context axioms_valid_ty)
+lemmas axioms_valid = axioms_valid_context axioms_valid_ty axioms_valid_tm
+
 (* context validity *)
-lemma context_valid_ty: "\<Gamma> \<turnstile>\<^sub>t\<^sub>y \<tau> : \<kappa> \<Longrightarrow> \<turnstile> \<Gamma>"
-  by (induction \<Gamma> \<tau> \<kappa> rule: Ty_induct) auto
-lemma context_valid_tm: "\<Gamma> \<turnstile> e : \<tau> \<Longrightarrow> \<turnstile> \<Gamma>"
-  by (induction \<Gamma> e \<tau> rule: Tm.induct) (auto simp: context_valid_ty)
+lemma context_valid_ty: "\<Gamma> , \<Delta> \<turnstile>\<^sub>t\<^sub>y \<tau> : \<kappa> \<Longrightarrow> \<Delta> \<turnstile> \<Gamma>"
+  by (induction \<Gamma> \<Delta> \<tau> \<kappa> rule: Ty_induct) auto
+lemma context_valid_tm: "\<Gamma> , \<Delta> \<turnstile> e : \<tau> \<Longrightarrow> \<Delta> \<turnstile> \<Gamma>"
+  by (induction \<Gamma> \<Delta> e \<tau> rule: Tm.induct) (auto simp: context_valid_ty)
 lemmas context_valid = context_valid_ty context_valid_tm
 
 (* \<lbrakk> \<Gamma> \<turnstile> e : t ; atom x \<sharp> \<Gamma> \<rbrakk> \<Longrightarrow> atom x \<sharp> e *)
-lemma fresh_in_context_ty: "\<lbrakk> \<Gamma> \<turnstile>\<^sub>t\<^sub>y \<tau> : k ; atom (a::tyvar) \<sharp> \<Gamma> \<rbrakk> \<Longrightarrow> atom a \<sharp> \<tau>"
-proof (induction \<Gamma> \<tau> k rule: Ty_induct)
-  case (Var \<Gamma> a k)
+lemma fresh_in_context_ty: "\<lbrakk> \<Gamma> , \<Delta> \<turnstile>\<^sub>t\<^sub>y \<tau> : k ; atom (a::tyvar) \<sharp> \<Gamma> \<rbrakk> \<Longrightarrow> atom a \<sharp> \<tau>"
+proof (induction \<Gamma> \<Delta> \<tau> k rule: Ty_induct)
+  case (Var \<Gamma> \<Delta> a k)
   then show ?case using fresh_at_base(2) fresh_not_isin_tyvar by fastforce
 qed (auto simp: fresh_Cons)
 
-lemma fresh_in_context_term_var: "\<lbrakk> \<Gamma> \<turnstile> e : \<tau> ; atom (x::var) \<sharp> \<Gamma> \<rbrakk> \<Longrightarrow> atom x \<sharp> e"
-proof (induction \<Gamma> e \<tau> rule: Tm.induct)
-case (Tm_Var \<Gamma> x \<tau>)
+lemma fresh_in_context_term_var: "\<lbrakk> \<Gamma> , \<Delta> \<turnstile> e : \<tau> ; atom (x::var) \<sharp> \<Gamma> \<rbrakk> \<Longrightarrow> atom x \<sharp> e"
+proof (induction \<Gamma> \<Delta> e \<tau> rule: Tm.induct)
+case (Tm_Var \<Gamma> \<Delta> x \<tau>)
   then show ?case using fresh_ineq_at_base fresh_not_isin_var by force
 qed (auto simp: fresh_Cons)
 
-lemma fresh_in_context_term_tyvar: "\<lbrakk> \<Gamma> \<turnstile> e : \<tau> ; atom (a::tyvar) \<sharp> \<Gamma> \<rbrakk> \<Longrightarrow> atom a \<sharp> e"
-proof (induction \<Gamma> e \<tau> rule: Tm.induct)
-  case (Tm_Abs \<Gamma> x \<tau>1 e \<tau>2)
-  then show ?case using Tm_Abs context_valid_tm fresh_Cons fresh_in_context_ty by fastforce
+lemma fresh_in_context_term_tyvar: "\<lbrakk> \<Gamma> , \<Delta> \<turnstile> e : \<tau> ; atom (a::tyvar) \<sharp> \<Gamma> \<rbrakk> \<Longrightarrow> atom a \<sharp> e"
+proof (induction \<Gamma> \<Delta> e \<tau> rule: Tm.induct)
+  case (Tm_Abs x \<tau>1 \<Gamma> \<Delta> e \<tau>2)
+  then have "atom a \<sharp> \<tau>1" by (meson CtxE(2) context_valid_tm fresh_in_context_ty)
+  then show ?case by (simp add: Tm_Abs fresh_Cons)
 next
   case (Tm_Let \<Gamma> e1 e2 \<tau>1 \<tau>2 x)
   then show ?case
-    by (metis (mono_tags, lifting) CtxE(2) binder.fresh(1) context_valid_tm fresh_Cons fresh_in_context_ty fresh_ineq_at_base list.set_intros(1) term.fresh(7))
+    by (metis (mono_tags, lifting) CtxE(2) binder.fresh(1) context_valid_tm fresh_Cons fresh_in_context_ty fresh_ineq_at_base list.set_intros(1) term_elist.fresh(7))
 qed (auto simp: fresh_Cons fresh_in_context_ty)
 lemmas fresh_in_context = fresh_in_context_ty fresh_in_context_term_var fresh_in_context_term_tyvar
 
-nominal_inductive Ctx avoids
+lemma fresh_in_axioms: "\<turnstile> \<Delta> \<Longrightarrow> atom (a::tyvar) \<sharp> \<Delta>"
+proof -
+  fix \<Gamma> \<tau> k
+  assume a: "\<turnstile> \<Delta>"
+  let ?Q = "\<lambda>b c d e. atom a \<sharp> c"
+  let ?W = "\<lambda>b c. atom a \<sharp> b"
+
+  have "(\<turnstile> \<Delta> \<longrightarrow> atom a \<sharp> \<Delta>) \<and> (\<Delta> \<turnstile> \<Gamma> \<longrightarrow> ?W \<Delta> \<Gamma>) \<and> (\<Gamma> , \<Delta> \<turnstile>\<^sub>t\<^sub>y \<tau> : k \<longrightarrow> ?Q \<Gamma> \<Delta> \<tau> k)"
+  proof (induction rule: Ax_Ctx_Ty.induct[of "\<lambda>x. atom a \<sharp> x" ?Q ?W])
+    case (Ax_Ctor \<Delta> \<tau> D)
+    then show ?case using fresh_in_context(1)[OF Ax_Ctor(1) fresh_Nil] fresh_Cons fresh_Nil by fastforce
+  qed (auto simp: fresh_Nil fresh_Cons)
+
+  then show ?thesis using a by simp
+qed
+
+lemma perm_axioms_tyvars[simp]: "\<turnstile> \<Delta> \<Longrightarrow> ((a::tyvar) \<leftrightarrow> b) \<bullet> \<Delta> = \<Delta>"
+  using flip_fresh_fresh fresh_in_axioms by blast
+
+nominal_inductive Ax avoids
   Ty_Forall: a
-proof (goal_cases)
-  case (1 a k \<Gamma> \<sigma>)
-  then have "\<turnstile> BTyVar a k # \<Gamma>" by (rule context_valid(1))
-  then have 1: "atom a \<sharp> \<Gamma>" by blast
-  obtain c \<sigma>' where 2: "(\<forall> a:k. \<sigma>) = (\<forall> c:k. \<sigma>') \<and> atom a \<sharp> (\<forall> c:k. \<sigma>')" using Abs_fresh_var by auto
-  then have "atom a \<sharp> (\<Gamma>, \<forall> c:k. \<sigma>', \<star>)" using 1 fresh_Pair by simp
+proof goal_cases
+  case (1 a k \<Gamma> \<Delta> \<sigma>)
+  then have "\<Delta> \<turnstile> BTyVar a k # \<Gamma>" by (rule context_valid(1))
+  then have 2: "atom a \<sharp> \<Gamma>" by blast
+  have 3: "atom a \<sharp> \<Delta>" by (rule fresh_in_axioms[OF axioms_valid(2)[OF 1]])
+  obtain c \<sigma>' where 4: "(\<forall> a:k. \<sigma>) = (\<forall> c:k. \<sigma>') \<and> atom a \<sharp> (\<forall> c:k. \<sigma>')" using Abs_fresh_var by auto
+  then have "atom a \<sharp> (\<Gamma>, \<Delta>, \<forall> c:k. \<sigma>', \<star>)" using 2 3 fresh_Pair by simp
   then show ?case using 2 fresh_star_def by fastforce
 qed auto
 
@@ -168,50 +290,30 @@ nominal_inductive Tm avoids
   Tm_Abs: x
   | Tm_TAbs: a
   | Tm_Let: x
-proof (goal_cases)
-  case (1 x \<tau>1 \<Gamma> e \<tau>2)
-  then have "\<turnstile> BVar x \<tau>1 # \<Gamma>" by (rule context_valid)
-  then have 1: "atom x \<sharp> \<Gamma>" by blast
-  obtain y e' where 2: "(\<lambda> x:\<tau>1. e) = (\<lambda> y:\<tau>1. e') \<and> atom x \<sharp> (\<lambda> y:\<tau>1. e')" using Abs_fresh_var by auto
-  then have "atom x \<sharp> (\<Gamma>, \<lambda> y:\<tau>1. e', \<tau>1 \<rightarrow> \<tau>2)" using 1 fresh_Pair by simp
-  then show ?case using 2 fresh_star_def by fastforce
+proof goal_cases
+  case (1 x \<tau>1 \<Gamma> \<Delta> e \<tau>2)
+  then have "\<Delta> \<turnstile> BVar x \<tau>1 # \<Gamma>" by (rule context_valid)
+  then have 2: "atom x \<sharp> \<Gamma>" by blast
+  obtain y e' where 4: "(\<lambda> x:\<tau>1. e) = (\<lambda> y:\<tau>1. e') \<and> atom x \<sharp> (\<lambda> y:\<tau>1. e')" using Abs_fresh_var by auto
+  then have "atom x \<sharp> (\<Gamma>, \<Delta>, \<lambda> y:\<tau>1. e', \<tau>1 \<rightarrow> \<tau>2)" using 2 fresh_Pair by simp
+  then show ?case using 4 fresh_star_def by fastforce
 next
-  case (3 a k \<Gamma> e \<sigma>)
-  then have "\<turnstile> BTyVar a k # \<Gamma>" by (rule context_valid)
+  case (3 a k \<Gamma> \<Delta> e \<sigma>)
+  then have "\<Delta> \<turnstile> BTyVar a k # \<Gamma>" by (rule context_valid)
   then have 1: "atom a \<sharp> \<Gamma>" by blast
-  obtain y e' where 2: "(\<Lambda> a:k. e) = (\<Lambda> y:k. e') \<and> atom a \<sharp> (\<Lambda> y:k. e')" using Abs_fresh_var by auto
-  obtain y2 \<sigma>' where 3: "(\<forall> a:k. \<sigma>) = (\<forall> y2:k. \<sigma>') \<and> atom a \<sharp> (\<forall> y2:k. \<sigma>')" using Abs_fresh_var by auto
-  then have "atom a \<sharp> (\<Gamma>, \<Lambda> y:k. e', \<forall> y2:k. \<sigma>')" using 1 2 by auto
-  then show ?case using 2 3 fresh_star_def by force
+  have 2: "atom a \<sharp> \<Delta>" by (rule fresh_in_axioms[OF axioms_valid(3)[OF 3]])
+  obtain y e' where 3: "(\<Lambda> a:k. e) = (\<Lambda> y:k. e') \<and> atom a \<sharp> (\<Lambda> y:k. e')" using Abs_fresh_var by auto
+  obtain y2 \<sigma>' where 4: "(\<forall> a:k. \<sigma>) = (\<forall> y2:k. \<sigma>') \<and> atom a \<sharp> (\<forall> y2:k. \<sigma>')" using Abs_fresh_var by auto
+  then have "atom a \<sharp> (\<Gamma>, \<Delta>, \<Lambda> y:k. e', \<forall> y2:k. \<sigma>')" using 1 2 3 by auto
+  then show ?case using 3 4 fresh_star_def by force
 next
-  case (5 \<Gamma> e1 \<tau>1 x e2 \<tau>2)
-  from 5(2) have "\<turnstile> BVar x \<tau>1 # \<Gamma>" by (rule context_valid)
+  case (5 \<Gamma> \<Delta> e1 \<tau>1 x e2 \<tau>2)
+  from 5(2) have "\<Delta> \<turnstile> BVar x \<tau>1 # \<Gamma>" by (rule context_valid)
   then have 1: "atom x \<sharp> \<Gamma>" by blast
   then have "atom x \<sharp> e1" using 5(1) fresh_in_context(2) by blast
   then obtain y e2' where 2: "Let x \<tau>1 e1 e2 = Let y \<tau>1 e1 e2' \<and> atom x \<sharp> Let y \<tau>1 e1 e2'" using Abs_fresh_var by auto
-  then have "atom x \<sharp> (\<Gamma>, Let y \<tau>1 e1 e2', \<tau>2)" using 1 fresh_Pair by simp
+  then have "atom x \<sharp> (\<Gamma>, \<Delta>, Let y \<tau>1 e1 e2', \<tau>2)" using 1 fresh_Pair by simp
   then show ?case using 2 fresh_star_def by fastforce
 qed auto
-
-(* Split strong induction principles *)
-lemma Ctx_strong_induct[consumes 1, case_names Empty TyVar Var]:
-  fixes c::"'a::fs"
-  assumes "\<turnstile> \<Gamma>"
-  and Empty: "\<And>c. P c []"
-  and TyVar: "\<And>\<Gamma> a k c. \<lbrakk> \<turnstile> \<Gamma> ; (\<And>c. P c \<Gamma>) ; atom a \<sharp> \<Gamma> \<rbrakk> \<Longrightarrow> P c (BTyVar a k # \<Gamma>)"
-  and Var: "\<And>\<Gamma> x \<tau> c. \<lbrakk> \<Gamma> \<turnstile>\<^sub>t\<^sub>y \<tau> : \<star> ; atom x \<sharp> \<Gamma> \<rbrakk> \<Longrightarrow> P c (BVar x \<tau> # \<Gamma>)"
-shows "P c \<Gamma>"
-  using assms(1) by (induction \<Gamma> rule: Ctx_Ty.strong_induct(1)[of _ P "\<lambda>c \<Gamma> \<tau> k. True"]) (auto simp: assms)
-
-lemma Ty_strong_induct[consumes 1, case_names Var App Unit FunArrow Forall]:
-  fixes c::"'a::fs"
-  assumes "\<Gamma> \<turnstile>\<^sub>t\<^sub>y \<tau> : \<kappa>"
-  and Var: "\<And>\<Gamma> a k c. \<lbrakk> \<turnstile> \<Gamma> ; BTyVar a k \<in> \<Gamma> \<rbrakk> \<Longrightarrow> P c \<Gamma> (TyVar a) k"
-  and App: "\<And>\<Gamma> \<tau>1 \<kappa>1 \<kappa>2 \<tau>2 c. \<lbrakk> \<Gamma> \<turnstile>\<^sub>t\<^sub>y \<tau>1 : KArrow \<kappa>1 \<kappa>2 ; (\<And>c. P c \<Gamma> \<tau>1 (KArrow \<kappa>1 \<kappa>2)) ; \<Gamma> \<turnstile>\<^sub>t\<^sub>y \<tau>2 : \<kappa>1 ; (\<And>c. P c \<Gamma> \<tau>2 \<kappa>1) \<rbrakk> \<Longrightarrow> P c \<Gamma> (TyConApp \<tau>1 \<tau>2) \<kappa>2"
-  and Unit: "\<And>\<Gamma> c. \<turnstile> \<Gamma> \<Longrightarrow> P c \<Gamma> TyUnit \<star>"
-  and FunArrow: "\<And>\<Gamma> \<tau>1 \<tau>2 c. \<lbrakk> \<Gamma> \<turnstile>\<^sub>t\<^sub>y \<tau>1 : \<star> ; (\<And>c. P c \<Gamma> \<tau>1 \<star>) ; \<Gamma> \<turnstile>\<^sub>t\<^sub>y \<tau>2 : \<star> ; (\<And>c. P c \<Gamma> \<tau>2 \<star>) \<rbrakk> \<Longrightarrow> P c \<Gamma> (\<tau>1 \<rightarrow> \<tau>2) \<star>"
-  and Forall: "\<And>a k \<Gamma> \<sigma> c. \<lbrakk> atom a \<sharp> c ; BTyVar a k # \<Gamma> \<turnstile>\<^sub>t\<^sub>y \<sigma> : \<star> ; (\<And>c. P c (BTyVar a k # \<Gamma>) \<sigma> \<star>) \<rbrakk> \<Longrightarrow> P c \<Gamma> (\<forall> a : k . \<sigma>) \<star>"
-shows "P c \<Gamma> \<tau> \<kappa>"
-  using assms(1) by (induction \<Gamma> \<tau> \<kappa> rule: Ctx_Ty.strong_induct(2)[of _ _ _ "\<lambda>c xs. True" P]) (auto simp: assms fresh_star_def)
 
 end
